Simple_Networks/Generalized_Network_Language_Impl.thy
@@ -1,0 +1,895 @@
+theory Generalized_Network_Language_Impl
+  imports
+    Generalized_Network_Language
+    TA_Impl.Normalized_Zone_Semantics_Impl_Refine
+    "HOL-Library.IArray" "HOL-Library.AList"
+    TA_Library.More_Methods
+    TA_Library.Bijective_Embedding
+    TA_Impl_Misc2
+    TA_More2
+    TA_Equivalences
+    "HOL-Eisbach.Eisbach_Tools"
+    TA_Library.TA_Syntax_Bundles
+    "Tag_Explorer"
+begin
+
+unbundle no_library_syntax
+
+paragraph \<open>Default maps\<close>
+
+definition default_map_of :: "'b \<Rightarrow> ('a \<times> 'b) list \<Rightarrow> 'a \<Rightarrow> 'b" where
+  "default_map_of a xs \<equiv> FinFun.map_default a (map_of xs)"
+
+lemma default_map_of_alt_def:
+  "default_map_of a xs x = (if x \<in> dom (map_of xs) then the (map_of xs x) else a)"
+  unfolding default_map_of_def map_default_def by (auto split: option.split_asm)
+
+lemma range_default_map_of:
+  "range (default_map_of x xs) \<subseteq> snd ` set xs \<union> {x}"
+  unfolding default_map_of_def map_default_def
+  by (auto split: option.split_asm) (meson img_snd map_of_SomeD)
+
+lemma finite_range_default_map_of:
+  "finite (range (default_map_of x m))"
+proof -
+  have "range (default_map_of x m) \<subseteq> the ` range (map_of m) \<union> {x}"
+    unfolding default_map_of_def FinFun.map_default_def
+    by (auto split: option.splits) (metis image_eqI option.sel rangeI)
+  also have "finite \<dots>"
+    by (blast intro: finite_range_map_of)
+  finally show ?thesis .
+qed
+
+lemma map_index'_inj:
+  "L = L'"
+  if "length L = length L'" "map_index' n f L = map_index' n g L'" "set L \<subseteq> S" "set L' \<subseteq> T"
+     "\<forall> i < length L + n. \<forall> x \<in> S. \<forall>y \<in> T. f i x = g i y \<longrightarrow> x = y"
+  using that
+proof (induction "length L" arbitrary: L L' n)
+  case 0
+  then show ?case
+    by simp
+next
+  case (Suc x)
+  from Suc.prems obtain a b L1 L1' where *:
+    "length L1 = x" "length L1' = x" "L = a # L1" "L' = b # L1'"
+    by (smt Suc.hyps(2) length_Suc_conv)
+  show ?case
+    unfolding \<open>L = _\<close> \<open>L' = _\<close>
+    apply (clarsimp, rule conjI)
+    subgoal
+      by (smt *(3,4) Suc.hyps(2) Suc.prems Suc_less_eq add_Suc_shift less_add_Suc2
+            list.set_intros(1) list_tail_coinc map_index'.simps(2) set_mp)
+    subgoal
+      apply (rule Suc.hyps)
+      using Suc.prems * by auto
+    done
+qed
+
+lemma map_index_inj:
+  "L = L'"
+  if "map_index f L = map_index g L'" "set L \<subseteq> S" "set L' \<subseteq> T"
+     "\<forall> i < length L. \<forall> x \<in> S. \<forall>y \<in> T. f i x = g i y \<longrightarrow> x = y"
+  using that by - (rule map_index'_inj, auto dest: map_index_eq_imp_length_eq)
+
+lemma map_index_inj1:
+  "L = L'"
+  if "map_index f L = map_index g L'"
+     "\<forall> i < length L. f i (L ! i) = g i (L' ! i) \<longrightarrow> L ! i = L' ! i"
+proof (intros add: nth_equalityI)
+  from that(1) show \<open>length L = length L'\<close>
+    by (rule map_index_eq_imp_length_eq)
+  fix i :: \<open>nat\<close>
+  assume \<open>i < length L\<close>
+  with that have "map_index f L ! i = map_index g L' ! i"
+    by auto
+  with \<open>i < length L\<close> \<open>length L = length L'\<close> have "f i (L ! i) = g i (L' ! i)"
+    by simp
+  with \<open>i < length L\<close> that(2) show \<open>L ! i = L' ! i\<close>
+    by simp
+qed
+
+lemma map_index_update:
+  "map_index f (xs[i := a]) = (map_index f xs)[i := f i a]"
+  by (rule nth_equalityI) (auto simp: nth_list_update')
+
+lemma map_trans_broad_aux1:
+  "map_index map_loc (fold (\<lambda>p L. L[p := ls' p]) ps L) =
+  fold (\<lambda>p L. L[p := map_loc p (ls' p)]) ps (map_index map_loc L)"
+  by (induction ps arbitrary: L) (auto simp: map_index_update)
+
+lemma ComD2:
+  fixes map_action
+  assumes "inj map_action" "Com (map_action a) = map_act map_action a'"
+  shows "a' = Com a"
+  using assms(2) by (cases a')  (auto simp: injD[OF assms(1)])
+
+lemma SilD2:
+  fixes map_action
+  assumes "inj map_action" "Sil (map_action a) = map_act map_action a'"
+  shows "a' = Sil a"
+  using assms(2) by (cases a')  (auto simp: injD[OF assms(1)])
+
+lemma (in Prod_TA_Defs) trans_sync_tagged_def:
+  "trans_sync =
+    {((L, s), concat (map gs ps), Sync sync, concat (map rs ps), (L', s')) |
+    sync L s L' s' bs gs as fs rs ls' ps.
+      ''sync'' \<bbar> sync \<in> syncs \<and>
+      ''enabled'' \<bbar> (\<forall>(p, a, b) \<in> set sync. b \<longrightarrow> p \<in> set ps) \<and>
+      ''only syncs'' \<bbar> (\<forall>p < n_ps. p \<notin> fst ` set sync \<longrightarrow> p \<notin> set ps) \<and>
+      ''actions'' \<bbar> (\<forall>(p, a, _) \<in> set sync. as p = a) \<and>
+      TRANS ''sync'' \<bbar>
+        (\<forall>p \<in> set ps. (L ! p, bs p, gs p, Com (as p), fs p, rs p, ls' p) \<in> trans (N p)) \<and>
+      ''committed'' \<bbar>
+        ((\<exists>p \<in> set ps. L ! p \<in> committed (N p)) \<or> (\<forall>p < n_ps. L ! p \<notin> committed (N p))) \<and>
+      ''maximal'' \<bbar> (\<forall>q < n_ps. q \<notin> set ps \<longrightarrow>
+        \<not> (\<exists>b g a f r l'.
+            (L!q, b, g, Com a, f, r, l') \<in> trans (N q) \<and> (q, a, False) \<in> set sync
+          \<and> check_bexp s b True)) \<and>
+      SEL ''range'' \<bbar> set ps \<subseteq> {0..<n_ps} \<and> SEL ''sublist'' \<bbar> subseq ps (map fst sync) \<and>
+      ''bexp'' \<bbar> (\<forall>p \<in> set ps. check_bexp s (bs p) True) \<and>
+      ''new loc'' \<bbar> L' = fold (\<lambda>p L . L[p := ls' p]) ps L \<and>
+      ''upds''    \<bbar> is_upds s (map fs ps) s' \<and>
+      L \<in> states \<and> ''bounded'' \<bbar> bounded bounds s \<and> ''bounded'' \<bbar> bounded bounds s'
+    }"
+  unfolding trans_sync_def by untag standard
+
+lemma (in Prod_TA_Defs) trans_sync_alt_def:
+  "trans_sync =
+    {((L, s), concat (map gs ps), Sync sync, concat (map rs ps), (L', s')) |
+    sync L s L' s' bs gs as fs rs ls' ps.
+      ''sync'' \<bbar> sync \<in> syncs \<and>
+      ''enabled'' \<bbar> (\<forall>(p, a, b) \<in> set sync. b \<longrightarrow> p \<in> set ps) \<and>
+      ''only syncs'' \<bbar> (\<forall>p < n_ps. p \<notin> fst ` set sync \<longrightarrow> p \<notin> set ps) \<and>
+      ''actions'' \<bbar> (\<forall>(p, a, _) \<in> set sync. as p = a) \<and>
+      TRANS ''sync'' \<bbar>
+        (\<forall>p \<in> set ps. (L ! p, bs p, gs p, Com (as p), fs p, rs p, ls' p) \<in> trans (N p)) \<and>
+      ''committed'' \<bbar>
+        ((\<exists>p \<in> set ps. L ! p \<in> committed (N p)) \<or> (\<forall>p < n_ps. L ! p \<notin> committed (N p))) \<and>
+      ''maximal'' \<bbar> (\<forall>q < n_ps. q \<notin> set ps \<longrightarrow>
+        \<not> (\<exists>b g a f r l'.
+            (L!q, b, g, Com a, f, r, l') \<in> trans (N q) \<and> (q, a, False) \<in> set sync
+          \<and> check_bexp s b True)) \<and>
+      SEL ''range'' \<bbar> set ps \<subseteq> {0..<n_ps} \<and> SEL ''sublist'' \<bbar> subseq ps (map fst sync) \<and>
+      ''bexp'' \<bbar> (\<forall>p \<in> set ps. check_bexp s (bs p) True) \<and>
+      ''new loc'' \<bbar> L' = fold (\<lambda>p L . L[p := ls' p]) ps L \<and>
+      ''upds''    \<bbar> is_upds s (map fs ps) s' \<and>
+      L \<in> states \<and> ''bounded'' \<bbar> bounded bounds s \<and> ''bounded'' \<bbar> bounded bounds s' \<and>
+      ''fix conds''  \<bbar> (\<forall>p. p\<notin>set ps \<longrightarrow> bs p = bexp.true) \<and>
+      ''fix guards'' \<bbar> (\<forall>p. p\<notin>set ps \<longrightarrow> gs p = []) \<and>
+      ''fix upds''   \<bbar> (\<forall>p. p\<notin>set ps \<longrightarrow> fs p = []) \<and>
+      ''fix resets'' \<bbar> (\<forall>p. p\<notin>set ps \<longrightarrow> rs p = [])
+    }"
+  unfolding trans_sync_tagged_def
+proof ((intro Collect_eqI iffI; elims add: more_elims), goal_cases)
+  case prems: (1 x sync L s L' s' bs gs as fs rs ls' ps)
+  let ?f = "\<lambda>gs p. if p \<in> set ps then gs p else []"
+  let ?bs = "\<lambda>p. if p \<in> set ps then bs p else bexp.true"
+  let ?gs = "?f gs" let ?fs = "?f fs" let ?rs = "?f rs"
+  have [simp]: "map gs ps = map ?gs ps" "map rs ps = map ?rs ps" "map fs ps = map ?fs ps"
+    by (simp cong: map_cong)+
+  with prems show ?case
+    by (inst_existentials sync L s L' s' ?bs ?gs as ?fs ?rs ls' ps) (tag, (assumption | simp))+
+qed blast
+
+
+definition
+  "conv_automaton \<equiv> \<lambda>(committed, urgent, trans, inv).
+    (committed,
+     urgent,
+     map (\<lambda>(l, b, g, a, f, r, l'). (l, b, conv_cc g, a, f, r, l')) trans,
+     map (\<lambda>(s, cc). (s, conv_cc cc)) inv)"
+
+definition
+  "automaton_of \<equiv>
+    \<lambda>(committed, urgent, trans, inv). (set committed, set urgent, set trans, default_map_of [] inv)"
+
+locale Simple_Network_Impl_Defs =
+  fixes automata ::
+    "('s list \<times> 's list \<times> ('a act, 's, 'c, 't, 'x, int) transition list
+      \<times> ('s \<times> ('c, 't) cconstraint) list) list"
+    and syncs :: "(nat \<times> 'a \<times> bool) list list"
+    and bounds' :: "('x \<times> (int \<times> int)) list"
+begin
+
+definition \<comment>\<open>Number of state variables\<close>
+  "n_vs = length bounds'"
+
+definition
+  "B x \<equiv> if x \<in> dom (map_of bounds') then the (map_of bounds' x) else (0, 0)"
+
+sublocale Prod_TA_Defs
+  "(set syncs, map automaton_of automata, map_of bounds')" .
+
+lemma L_len[intro, dest]:
+  "length L = n_ps" if "L \<in> states"
+  using that unfolding states_def by simp
+
+end
+
+(*
+locale Simple_Network_Impl =
+  Simple_Network_Impl_Defs automata broadcast bounds
+  for
+    automata ::
+    "('s list \<times> ('a act, 's, 'c, int, 'x, int) transition list
+      \<times> ('s \<times> ('c, int) cconstraint) list) list"
+  and broadcast bounds
+*)
+
+locale Simple_Network_Impl =
+  fixes automata ::
+    "('s list \<times> 's list \<times> ('a act, 's, 'c, int, 'x, int) transition list
+      \<times> ('s \<times> ('c, int) cconstraint) list) list"
+    and syncs :: "(nat \<times> 'a \<times> bool) list list"
+    and bounds' :: "('x \<times> (int \<times> int)) list"
+begin
+
+sublocale Simple_Network_Impl_Defs automata syncs bounds' .
+
+end
+
+
+paragraph \<open>Mapping through the product construction\<close>
+
+lemma f_the_inv_f:
+  "f (the_inv f x) = x" if "inj f" "x \<in> range f"
+  using that by (auto simp: the_inv_f_f)
+
+context Simple_Network_Impl
+begin
+
+lemma N_eq:
+  \<open>N i = automaton_of (automata ! i)\<close> if \<open>i < n_ps\<close>
+  using that unfolding N_def n_ps_def fst_conv snd_conv by (intro nth_map; simp)
+
+(* XXX Remove? *)
+lemma covn_N_eq:
+  \<open>N i = automaton_of (automata ! i)\<close> if \<open>i < n_ps\<close>
+  using that unfolding N_def n_ps_def fst_conv snd_conv by (intro nth_map; simp)
+
+end
+
+inductive_cases check_bexp_elims:
+  "check_bexp s bexp.true bv"
+  "check_bexp s (bexp.not b) bv"
+  "check_bexp s (bexp.and b1 b2) bv"
+  "check_bexp s (bexp.or b1 b2) bv"
+  "check_bexp s (bexp.imply b1 b2) bv"
+  "check_bexp s (le i x) bv"
+  "check_bexp s (lt i x) bv"
+  "check_bexp s (ge i x) bv"
+  "check_bexp s (eq i x) bv"
+  "check_bexp s (gt i x) bv"
+
+inductive_cases is_val_elims:
+  "is_val s (const c) d"
+  "is_val s (var x)   v"
+  "is_val s (if_then_else b e1 e2) v"
+  "is_val s (binop f e1 e2) v"
+  "is_val s (unop f e) v"
+
+method fprem =
+  (match premises in R: _ \<Rightarrow> \<open>rule R[elim_format]\<close>, assumption)
+
+context Simple_Network_Impl
+begin
+
+paragraph \<open>Conversion from integers to reals commutes with product construction.\<close>
+
+sublocale conv: Prod_TA_Defs
+  "(set syncs, map (Generalized_Network_Language.conv_A o automaton_of) automata, map_of bounds')" .
+
+lemma (in -) conv_ac_inj:
+  "ac = ac'" if "conv_ac ac = conv_ac ac'"
+  using that by (cases ac; cases ac'; auto)
+
+lemma (in -) conv_cc_inj:
+  "cc = cc'" if "conv_cc cc = conv_cc cc'"
+  using that by (subst (asm) inj_map_eq_map) (auto simp add: conv_ac_inj intro: injI)
+
+context
+begin
+
+lemma conv_alt_def:
+  "conv (set syncs, map automaton_of automata, map_of bounds') =
+    (set syncs, map (Generalized_Network_Language.conv_A o automaton_of) automata, map_of bounds')"
+  unfolding conv_def by simp
+
+private lemma 2:
+  "Generalized_Network_Language.conv_A o automaton_of = (\<lambda>(committed, urgent, trans, inv).
+    (set committed,
+     set urgent,
+     set (map Generalized_Network_Language.conv_t trans),
+     default_map_of [] (map (\<lambda> (l, g). (l, conv_cc g)) inv)))"
+  apply (rule ext)
+  apply clarsimp
+  unfolding Generalized_Network_Language.conv_A_def automaton_of_def
+  apply (clarsimp split: prod.split)
+  unfolding default_map_of_def
+  unfolding FinFun.map_default_def
+  apply (rule ext)
+  subgoal for xs a
+    by (induction xs) auto
+  done
+
+lemma conv_n_ps_eq:
+  "conv.n_ps = n_ps"
+  by (simp add: Prod_TA_Defs.n_ps_def)
+
+lemma conv_N_eq:
+  "conv.N i = Generalized_Network_Language.conv_A (N i)" if "i < n_ps"
+  using that unfolding n_ps_def Prod_TA_Defs.N_def fst_conv snd_conv by (subst nth_map | simp)+
+
+private lemma 5:
+  "inv (conv.N i) = conv_cc o (inv (N i))" if "i < n_ps"
+  unfolding conv_N_eq[OF that] unfolding Generalized_Network_Language.conv_A_def
+  by (simp split: prod.split add: inv_def)
+
+lemma trans_conv_N_eq:
+  "trans (conv.N i) = Generalized_Network_Language.conv_t ` (trans (N i))"  if "i < n_ps"
+  unfolding conv_N_eq[OF that] unfolding Generalized_Network_Language.conv_A_def
+  by (simp split: prod.split add: trans_def)
+
+private lemma 71:
+  "(l, b, conv_cc g, a, r, u, l')\<in>Simple_Network_Language.trans (conv.N i)"
+  if "(l, b, g, a, r, u, l')\<in>Simple_Network_Language.trans (N i)" "i < n_ps"
+  using that by (force simp add: trans_conv_N_eq Generalized_Network_Language.conv_t_def)
+
+private lemma 72:
+  "(l, b, conv_cc g, a, r, u, l')\<in>Simple_Network_Language.trans (conv.N i)
+\<longleftrightarrow> (l, b, g, a, r, u, l')\<in>Simple_Network_Language.trans (N i)" if "i < n_ps"
+  by (auto simp: trans_conv_N_eq[OF that] Generalized_Network_Language.conv_t_def
+           dest: conv_cc_inj intro: image_eqI[rotated])
+
+private lemma 73:
+  "\<exists>g'. g = conv_cc g' \<and> (l, b, g', a, r, u, l')\<in>Simple_Network_Language.trans (N i)"
+  if "(l, b, g, a, r, u, l')\<in>Simple_Network_Language.trans (conv.N i)" "i < n_ps"
+  using that by (force simp: trans_conv_N_eq Generalized_Network_Language.conv_t_def)
+
+lemma conv_bounds[simp]:
+  "conv.bounds = bounds"
+  unfolding conv.bounds_def bounds_def by simp
+
+lemma conv_states[simp]:
+  "conv.states = states"
+  unfolding conv.states_def states_def conv_n_ps_eq
+  by (auto simp add: trans_conv_N_eq Generalized_Network_Language.conv_t_def) (fastforce, force)
+
+private lemma 9:
+  "committed (conv.N p) = committed (N p)" if \<open>p < n_ps\<close>
+  unfolding conv_N_eq[OF that] unfolding Generalized_Network_Language.conv_A_def
+  by (simp split: prod.split add: committed_def)
+
+private lemma 10:
+  "conv.syncs = set syncs"
+  unfolding conv.syncs_def by simp
+
+lemma conv_trans_int:
+  "conv.trans_int = (\<lambda>(l, g, a, r, l'). (l, map conv_ac g, a, r, l')) ` trans_int"
+  unfolding conv.trans_int_def trans_int_def
+  supply [simp] = L_len
+  apply standard
+  subgoal
+    by (clarsimp simp: Generalized_Network_Language.conv_t_def conv_n_ps_eq trans_conv_N_eq 9)
+      (intros add: more_intros, solve_triv+)
+  subgoal
+    by (rule subsetI,
+        clarsimp simp: Generalized_Network_Language.conv_t_def conv_n_ps_eq trans_conv_N_eq 9[symmetric])
+      ((drule (1) 71)+, intros add: more_intros, solve_triv+)
+  done
+
+lemma n_ps_rangeD:
+  "p < n_ps" if "p \<in> set ps" "set ps \<subseteq> {0..<n_ps}"
+  using that by auto
+
+lemma conv_trans_sync:
+  "conv.trans_sync = (\<lambda>(l, g, a, r, l'). (l, map conv_ac g, a, r, l')) ` trans_sync"
+  unfolding conv.trans_sync_alt_def trans_sync_alt_def
+  apply standard
+  supply [simp] = L_len
+  subgoal
+  proof -
+    have **: "\<exists> gs'. gs = conv_cc o gs' \<and>
+          (\<forall>p\<in>set ps.(L ! p, bs p, gs' p, Com (as p), fs p, rs p, ls' p) \<in> trans (N p))"
+      if assms[untagged]:
+        "\<forall>p\<in>set ps. (L ! p, bs p, gs p, Com (as p), fs p, rs p, ls' p) \<in> trans (conv.N p)"
+        "SEL ''range'' \<bar> set ps \<subseteq> {0..<n_ps}" "''fix guards'' \<bar> \<forall>p. p \<notin> set ps \<longrightarrow> gs p = []"
+      for L ps bs gs as fs rs ls'
+    proof -
+      have *: "gs p = conv_cc (Hilbert_Choice.inv conv_cc (gs p))" if "p \<in> set ps" for p
+        using that assms by (auto 4 3 simp: f_inv_into_f dest!: 73)
+      show ?thesis
+        apply (inst_existentials "Hilbert_Choice.inv conv_cc o gs")
+        subgoal
+          apply (rule ext)
+          subgoal for p
+            apply (cases "p \<in> set ps")
+            subgoal
+              by (simp, erule *)
+            subgoal
+              using assms(3) by (auto intro: injI inv_f_eq conv_ac_inj)
+            done
+          done
+        subgoal
+          using assms * by (force dest!: conv_cc_inj 73)
+        done
+    qed
+    show ?thesis
+      apply (rule subsetI)
+      apply (clarsimp simp add: conv_n_ps_eq 9 10 syncs_def split: prod.split_asm)
+      unfolding TAG_def[where t = "TRANS _"]
+      apply (drule **, (tag, assumption), (tag, assumption))
+      apply elims
+      apply (fo_rule image_eqI[rotated])
+      apply (intro CollectI exI conjI)
+      apply solve_triv
+      preferT \<open>''upds''\<close> \<comment> \<open>Start with this to get the right instantiation\<close>
+        apply (tag, assumption)
+      apply (all \<open>(tag, assumption)?\<close>)
+      preferT \<open>''enabled''\<close>
+        apply (tag, blast)
+      preferT \<open>''actions''\<close>
+        apply (tag, blast)
+      preferT \<open>''committed''\<close>
+        apply (tag- \<open>SEL ''range''\<close>, simp add: 9 subset_code(1); fail)
+      preferT \<open>''maximal''\<close>
+        apply (tag, blast dest: 71)
+      preferT \<open>''fix guards''\<close>
+        apply (tag, simp; fail)
+      subgoal \<comment> \<open>Equation from @{thm image_eqI}\<close>
+        apply (simp add: map_concat)
+        done
+      done
+  qed
+  subgoal
+    apply (rule subsetI)
+    apply (clarsimp simp: conv_n_ps_eq trans_conv_N_eq 10 syncs_def map_concat)
+    apply (intros add: more_intros)
+    apply solve_triv+
+    apply (tag- \<open>SEL ''range''\<close>, subst comp_def, fast elim: 71 intro: n_ps_rangeD; fail)
+    preferT \<open>''committed''\<close>
+      apply (tag- \<open>SEL ''range''\<close>, simp add: 9 subset_code(1); fail)
+    preferT \<open>''maximal''\<close>
+      apply (tag, simp add: Generalized_Network_Language.conv_t_def, fast; fail)
+    apply (tag, assumption)+
+    apply (tag, simp; fail)+
+  done
+done
+
+lemma conv_prod_ta:
+  "conv.prod_ta = Normalized_Zone_Semantics_Impl.conv_A prod_ta"
+  unfolding conv.prod_ta_def prod_ta_def
+  unfolding conv.trans_prod_def trans_prod_def
+  unfolding conv.prod_inv_def prod_inv_def
+  unfolding conv.N_def N_def conv_n_ps_eq
+  unfolding conv_A_def
+  apply simp
+  apply (rule conjI)
+  subgoal
+    unfolding image_Un
+    by ((fo_rule arg_cong2)+; rule conv_trans_int conv_trans_sync)
+  subgoal \<comment>\<open>Invariant\<close>
+    unfolding conv.N_def N_def
+    by (rule ext) (auto simp: 5 map_concat intro!: map_cong arg_cong[where f = concat])
+  done
+
+end (* Anonymous context for private lemmas *)
+
+paragraph \<open>Fundamentals\<close>
+
+definition "clkp_set' \<equiv>
+    (\<Union> A \<in> set automata. \<Union> g \<in> set (snd (snd (snd A))). collect_clock_pairs (snd g))
+  \<union> (\<Union> A \<in> set automata. \<Union> (l, b, g, _) \<in> set (fst (snd (snd A))). collect_clock_pairs g)"
+
+definition clk_set'  where
+  \<open>clk_set'  =
+  fst ` clkp_set' \<union>
+  (\<Union> A \<in> set automata. \<Union> (_, _, _, _, _, r, _) \<in> set (fst (snd (snd A))). set r)\<close>
+
+lemma (in -) default_map_of_in_listD:
+  "x \<in> \<Union> (set ` snd ` set invs)" if "x \<in> set (default_map_of [] invs l)"
+proof -
+  have "[] \<noteq> default_map_of [] invs l"
+    using that by force
+  then have "default_map_of [] invs l \<in> snd ` set invs"
+    by (metis (no_types) UNIV_I Un_insert_right range_default_map_of[of "[]" "invs"]
+          image_eqI insertE subsetCE sup_bot.right_neutral)
+  with that show ?thesis
+    by blast
+qed
+
+lemma collect_clock_pairs_invsI:
+  "(a, b) \<in> \<Union> ((collect_clock_pairs o snd) ` set invs)"
+  if "(a, b) \<in> collect_clock_pairs (default_map_of [] invs l)"
+  using that unfolding collect_clock_pairs_def by (auto dest!: default_map_of_in_listD)
+
+lemma mem_trans_N_iff:
+  "t \<in> Simple_Network_Language.trans (N i) \<longleftrightarrow> t \<in> set (fst (snd (snd (automata ! i))))"
+  if "i < n_ps"
+  unfolding N_eq[OF that] by (auto split: prod.splits simp: automaton_of_def trans_def)
+
+lemma length_automata_eq_n_ps:
+  "length automata = n_ps"
+  unfolding n_ps_def by simp
+
+lemma clkp_set'_subs:
+  "Timed_Automata.clkp_set prod_ta \<subseteq> clkp_set'"
+  unfolding Timed_Automata.clkp_set_def clkp_set'_def
+  apply (rule union_subsetI)
+  subgoal
+    unfolding Timed_Automata.collect_clki_def inv_of_prod prod_inv_def
+    apply (auto simp: collect_clock_pairs_concat)
+    apply (subst (asm) N_eq)
+     apply assumption
+    subgoal for a b L i
+      apply (inst_existentials "automata ! i")
+      subgoal
+        unfolding automaton_of_def
+        by (force dest!: nth_mem collect_clock_pairs_invsI
+            split: prod.split_asm simp: inv_def Prod_TA_Defs.n_ps_def)
+      done
+    done
+  subgoal
+    apply simp
+    unfolding trans_prod_def Timed_Automata.collect_clkt_def
+    apply safe
+    subgoal
+      unfolding trans_int_def by (fastforce simp: length_automata_eq_n_ps mem_trans_N_iff)
+    subgoal
+      unfolding trans_sync_tagged_def
+      by (clarsimp, tag- \<open>TRANS _\<close> \<open>SEL ''range''\<close>)
+         (fastforce simp: length_automata_eq_n_ps mem_trans_N_iff collect_clock_pairs_concat)
+      done
+    done
+
+lemma collect_clkvt_subs:
+  "collect_clkvt (trans_of prod_ta) \<subseteq>
+    (\<Union> A \<in> set automata. \<Union> (_, _, _, _, _, r, _) \<in> set (fst (snd (snd A))). set r)"
+  apply simp
+  unfolding collect_clkvt_def
+  apply auto
+  unfolding trans_prod_def
+  subgoal
+    apply simp
+    unfolding trans_prod_def Timed_Automata.collect_clkt_def
+    apply safe
+    subgoal
+      unfolding trans_int_def
+      by (fastforce
+          simp: length_automata_eq_n_ps mem_trans_N_iff
+          dest!: collect_clock_pairs_append_cases)
+    subgoal
+      unfolding trans_sync_tagged_def
+      by (clarsimp, tag- \<open>TRANS _\<close> \<open>SEL ''range''\<close>)
+         (fastforce simp: length_automata_eq_n_ps mem_trans_N_iff collect_clock_pairs_concat)
+    done
+  done
+
+lemma clk_set'_subs: "clk_set prod_ta \<subseteq> clk_set'"
+  using collect_clkvt_subs clkp_set'_subs unfolding clk_set'_def by auto
+
+end (* Simple Network Impl *)
+
+
+lemma (in Prod_TA_Defs) finite_range_invI:
+  "finite (range prod_inv)" if assms: "\<forall> i < n_ps. finite (range (inv (N i)))"
+proof -
+  let ?N = "\<Union> (range ` inv ` N ` {0..<n_ps})"
+  let ?X = "{I. set I \<subseteq> ?N \<and> length I \<le> n_ps}"
+  have "finite ?N"
+    using assms by auto
+  then have "finite ?X"
+    by (rule finite_lists_length_le)
+  moreover have "range prod_inv \<subseteq> concat ` ?X \<union> {[]}"
+  proof
+    fix x assume "x \<in> range prod_inv"
+    then consider L where "x = concat (map (\<lambda>p. (inv (N p)) (L ! p)) [0..<n_ps])" | "x = []"
+      unfolding prod_inv_def by (auto split: if_split_asm)
+    then show "x \<in> concat ` ?X \<union> {[]}"
+      by (cases; force)
+  qed
+  ultimately show ?thesis by - (drule finite_subset; auto)
+qed
+
+definition (in Prod_TA_Defs)
+  "loc_set =
+  (\<Union> {fst ` trans (N p) | p. p < n_ps} \<union>
+        \<Union> {(snd o snd o snd \<circ> snd \<circ> snd \<circ> snd) ` trans (N p) | p. p < n_ps})"
+
+lemma (in Prod_TA_Defs) states_loc_set:
+  "states \<subseteq> {L. set L \<subseteq> loc_set \<and> length L = n_ps}"
+  unfolding states_def loc_set_def
+  apply (intros add: more_intros)
+   apply (elims add: more_elims)
+   apply (drule mem_nth)
+   apply simp
+   apply (elims add: allE, assumption)
+   apply (simp split: prod.split_asm)
+   apply (erule disjE; (intros add: disjI1 disjI2 more_intros, solve_triv+); fail)
+  by (elims add: more_elims)
+
+lemma (in Prod_TA_Defs) finite_states:
+  assumes finite_trans: "\<forall>p < n_ps. finite (Simple_Network_Language.trans (N p))"
+  shows "finite states"
+proof -
+  have "states \<subseteq> {L. set L \<subseteq> loc_set \<and> length L = n_ps}"
+    by (rule states_loc_set)
+  also from finite_trans have "finite \<dots>"
+    unfolding loc_set_def by (intro finite_intros) auto
+  finally show ?thesis .
+qed
+
+context Simple_Network_Impl
+begin
+
+lemma trans_N_finite:
+  assumes "p < n_ps"
+  shows "finite (Simple_Network_Language.trans (N p))"
+  using assms by (subst N_eq) (auto simp: automaton_of_def trans_def split: prod.split)
+
+lemma states_finite:
+  "finite states"
+  by (intros add: finite_states trans_N_finite)
+
+lemma bounded_finite:
+  "finite {s. bounded bounds s}"
+proof -
+  let ?l = "Min {fst (the (bounds x)) | x. x \<in> dom bounds}"
+  let ?u = "Max {snd (the (bounds x)) | x. x \<in> dom bounds}"
+  have "finite (dom bounds)"
+    unfolding bounds_def by simp
+  then have "{s. bounded bounds s} \<subseteq> {s. dom s = dom bounds \<and> ran s \<subseteq> {?l..?u}}"
+    unfolding bounded_def
+    apply clarsimp
+    apply (rule conjI)
+    subgoal for s v
+      unfolding ran_is_image
+      apply clarsimp
+      subgoal for x l u
+        by (rule order.trans[where b = "fst (the (bounds x))"]; (rule Min_le)?; force)
+      done
+    subgoal for s v
+      unfolding ran_is_image
+      apply clarsimp
+      subgoal for x l u
+        by (rule order.trans[where b = "snd (the (bounds x))"]; (rule Max_ge)?; force)
+      done
+    done
+  also from \<open>finite (dom bounds)\<close> have "finite \<dots>"
+    by (rule finite_set_of_finite_maps) rule
+  finally show ?thesis .
+qed
+
+lemma trans_prod_finite:
+  "finite trans_prod"
+proof -
+  have "finite trans_int"
+  proof -
+    have "trans_int \<subseteq>
+      {((L, s), g, Internal a, r, (L', s')) | L s p l b g a f r l' s' L'.
+        L \<in> states \<and> bounded bounds s \<and> p < n_ps \<and>
+        (l, b, g, Sil a, f, r, l') \<in> trans (N p) \<and>
+        bounded bounds s'
+        \<and> L' = L[p := l']
+      }"
+      unfolding trans_int_def by (force simp: L_len)
+    also have "finite \<dots>"
+    proof -
+      have "finite {(a, b, c, d, e, f, g). (a, b, c, Sil d, e, f, g) \<in> trans (N p)}"
+        if "p < n_ps" for p
+        using [[simproc add: finite_Collect]] that
+        by (auto intro: trans_N_finite finite_vimageI injI)
+      with states_finite bounded_finite show ?thesis
+        by defer_ex
+    qed
+    finally show ?thesis .
+  qed
+  moreover have "finite trans_sync"
+  proof -
+    define P where "P sync ps \<equiv> set ps \<subseteq> {0..<n_ps} \<and> subseq ps (map fst sync)"
+      for ps and sync :: "(nat \<times> 'a \<times> bool) list"
+    define Q where "Q as n bs gs fs rs \<equiv>
+      (\<forall>p < n. \<exists> q < n_ps. \<exists> l l'. (l, bs ! p, gs ! p, as ! p, fs ! p, rs ! p, l') \<in> trans (N q)) \<and>
+              length as = n \<and> length bs = n \<and> length gs = n \<and> length fs = n \<and> length rs = n"
+      for as n bs gs fs rs
+    define tag where "tag x = True" for x :: 's
+    have Q_I: "Q (map as ps) (length ps) (map bs ps) (map gs ps) (map fs ps) (map rs ps)"
+      if "set ps \<subseteq> {0..<n_ps}"
+         "\<forall>p\<in>set ps. (L ! p, bs p, gs p, as p, fs p, rs p, ls' p) \<in> trans (N p)"
+      for ps :: "nat list" and L as bs gs fs rs ls'
+      using that unfolding Q_def by (auto 4 4 dest!: nth_mem)
+    have "trans_sync \<subseteq>
+      {((L, s), concat gs, Sync sync, concat rs, (L', s'')) |
+      L s sync ps as bs gs fs rs L' s''.
+        L \<in> states \<and> bounded bounds s \<and> \<^cancel>\<open>a \<in> set broadcast \<and>\<close> sync \<in> set syncs \<and>
+        \<^cancel>\<open>p < n_ps \<and>\<close>
+        \<^cancel>\<open>(l, b, g, Com a, f, r, l') \<in> trans (N p) \<and>\<close>
+        P sync ps \<and>
+        Q as (length ps) bs gs fs rs \<and>
+        L' \<in> states \<and>
+        bounded bounds s''\<^cancel>\<open> \<and>
+        tag l'\<close>
+    }"
+      unfolding trans_sync_def syncs_def
+      apply (rule subsetI)
+      apply (elims add: more_elims)
+      apply (intros add: more_intros)
+             apply solve_triv+
+         apply (unfold P_def; solve_triv)
+        apply (rule Q_I; assumption)
+      by (blast intro: state_preservation_updI state_preservation_fold_updI)
+    also have "finite \<dots>"
+    proof -
+      have "finite {(a, b, c, e, f, g). (a, b, c, Com d, e, f, g) \<in> trans (N p)}"
+        if "p < n_ps" for p d
+        using [[simproc add: finite_Collect]] that
+        by (auto intro: trans_N_finite finite_vimageI injI)
+      moreover have "finite {ps. P sync ps}" for sync
+        unfolding P_def by (simp add: finite_subseqs)
+      moreover have "finite {(as, bs, gs, fs, rs). Q as n bs gs fs rs}" (is "finite ?S") for n
+      proof -
+        let ?T = "\<Union> (trans ` N ` {0..<n_ps})"
+        have "?S \<subseteq> {(as, bs, gs, fs, rs).
+          (set as \<subseteq> (\<lambda>(_,_,_,a,_). a) ` ?T \<and> length as = n) \<and>
+          (set bs \<subseteq> (\<lambda>(_,b,_). b) ` ?T \<and> length bs = n) \<and>
+          (set gs \<subseteq> (\<lambda>(_,_,g,_). g) ` ?T \<and> length gs = n) \<and>
+          (set fs \<subseteq> (\<lambda>(_,_,_,_,f,_). f) ` ?T \<and> length fs = n) \<and>
+          (set rs \<subseteq> (\<lambda>(_,_,_,_,_,r,_). r) ` ?T \<and> length rs = n)
+        }"
+          unfolding Q_def by (safe; (drule mem_nth; elims; drule spec; elims; force))
+        also have "finite \<dots>"
+          using trans_N_finite by (intro finite_intros more_finite_intros) auto
+        finally show ?thesis .
+      qed
+      ultimately show ?thesis
+        using states_finite bounded_finite by defer_ex
+    qed
+    finally show ?thesis .
+  qed
+  ultimately show ?thesis
+    by (simp add: trans_prod_def)
+qed
+
+lemma prod_inv_finite:
+  "finite (range prod_inv)"
+  apply (intros add: finite_range_invI)
+  unfolding length_automata_eq_n_ps[symmetric]
+  unfolding N_def
+  unfolding automaton_of_def
+  by (auto intro: finite_range_default_map_of split: prod.split simp: inv_def)
+
+end (* Simple Network Impl *)
+
+paragraph \<open>Collecting variables from expressions.\<close>
+
+fun vars_of_bexp and vars_of_exp where
+  "vars_of_bexp (not e) = vars_of_bexp e"
+| "vars_of_bexp (and e1 e2) = (vars_of_bexp e1 \<union> vars_of_bexp e2)"
+| "vars_of_bexp (bexp.or e1 e2) = (vars_of_bexp e1 \<union> vars_of_bexp e2)"
+| "vars_of_bexp (imply e1 e2) = (vars_of_bexp e1 \<union> vars_of_bexp e2)"
+| "vars_of_bexp (eq i x) = vars_of_exp i \<union> vars_of_exp x"
+| "vars_of_bexp (le i x) = vars_of_exp i \<union> vars_of_exp x"
+| "vars_of_bexp (lt i x) = vars_of_exp i \<union> vars_of_exp x"
+| "vars_of_bexp (ge i x) = vars_of_exp i \<union> vars_of_exp x"
+| "vars_of_bexp (gt i x) = vars_of_exp i \<union> vars_of_exp x"
+| "vars_of_bexp bexp.true = {}"
+| "vars_of_exp (const c) = {}"
+| "vars_of_exp (var x) = {x}"
+| "vars_of_exp (if_then_else b e1 e2) = vars_of_bexp b \<union> vars_of_exp e1 \<union> vars_of_exp e2"
+| "vars_of_exp (binop _ e1 e2) = vars_of_exp e1 \<union> vars_of_exp e2"
+| "vars_of_exp (unop _ e) = vars_of_exp e"
+
+definition (in Prod_TA_Defs)
+  "var_set =
+  (\<Union>S \<in> {(fst \<circ> snd) ` trans (N p) | p. p < n_ps}. \<Union>b \<in> S. vars_of_bexp b) \<union>
+  (\<Union>S \<in> {(fst \<circ> snd \<circ> snd \<circ> snd \<circ> snd) ` trans (N p) | p. p < n_ps}.
+    \<Union>f \<in> S. \<Union> (x, e) \<in> set f. {x} \<union> vars_of_exp e)"
+
+locale Simple_Network_Impl_nat_defs =
+  Simple_Network_Impl automata
+  for automata ::
+    "(nat list \<times> nat list \<times> (nat act, nat, nat, int, nat, int) transition list
+      \<times> (nat \<times> (nat, int) cconstraint) list) list" +
+  fixes m :: nat and num_states :: "nat \<Rightarrow> nat" and num_actions :: nat
+
+locale Simple_Network_Impl_nat =
+  Simple_Network_Impl_nat_defs +
+  assumes has_clock: "m > 0"
+  assumes non_empty: "0 < length automata"
+    (* assumes "length automata = length state_nums" *)
+  assumes trans_num_states:
+    "\<forall>i < n_ps. let (_, _, trans, _) = (automata ! i) in \<forall> (l, _, _, _, _, _, l') \<in> set trans.
+      l < num_states i \<and> l' < num_states i"
+    and inv_num_states:
+    "\<forall>i < n_ps. let (_, _, _, inv) = (automata ! i) in \<forall> (x, _) \<in> set inv. x < num_states i"
+  assumes var_set:
+    "\<forall>(_, _, trans, _) \<in> set automata. \<forall>(_, _, _, _, f, _, _) \<in> set trans.
+      \<forall>(x, upd) \<in> set f. x < n_vs \<and> (\<forall>i \<in> vars_of_exp upd. i < n_vs)"
+    "\<forall>(_, _, trans, _) \<in> set automata. \<forall>(_, b, _, _, _, _, _) \<in> set trans.
+      \<forall>i \<in> vars_of_bexp b. i < n_vs"
+  assumes bounds:
+    "\<forall> i < n_vs. fst (bounds' ! i) = i"
+  assumes action_set:
+    "\<forall>sync \<in> set syncs. \<forall>(p, a, b) \<in> set sync. p < length automata \<and> a < num_actions"
+    "\<forall>(_, _, trans, _) \<in> set automata. \<forall>(_, _, _, a, _, _, _) \<in> set trans.
+        pred_act (\<lambda>a. a < num_actions) a"
+  assumes clock_set:
+    "\<forall>(_, _, trans, _) \<in> set automata. \<forall>(_, _, g, _, _, r, _) \<in> set trans.
+      (\<forall>c \<in> set r. 0 < c \<and> c \<le> m) \<and>
+      (\<forall> (c, x) \<in> collect_clock_pairs g. 0 < c \<and> c \<le> m \<and> x \<in> \<nat>)
+      "
+    "\<forall>(_, _, _, inv) \<in> set automata. \<forall>(l, g) \<in> set inv.
+      (\<forall> (c, x) \<in> collect_clock_pairs g. 0 < c \<and> c \<le> m \<and> x \<in> \<nat>)
+      "
+  assumes weak_synchronizations:
+    "\<forall>(_, _, trans, _) \<in> set automata. \<forall>(_, _, g, a, _, _, _) \<in> set trans. \<forall>sync \<in> set syncs.
+      case a of Com a \<Rightarrow> (p, a, False) \<in> set sync \<longrightarrow> g = [] | _ \<Rightarrow> True"
+begin
+
+lemma weak_synchronizations_unguarded:
+  "\<forall>p < n_ps. \<forall>sync l b g a f r l'. sync \<in> set syncs \<and>
+    (l, b, g, Com a, f, r, l') \<in> trans (N p) \<and> (p, a, False) \<in> set sync \<longrightarrow> g = []"
+  using weak_synchronizations by (fastforce dest: nth_mem simp: n_ps_def mem_trans_N_iff)
+
+sublocale conv: Prod_TA
+  "(set syncs, map (Generalized_Network_Language.conv_A o automaton_of) automata, map_of bounds')"
+  using weak_synchronizations_unguarded
+  by - (standard,
+        fastforce simp: conv.syncs_def Generalized_Network_Language.conv_t_def
+          conv_n_ps_eq trans_conv_N_eq)
+
+sublocale TA_Start_No_Ceiling prod_ta init m
+proof standard
+  show "finite (trans_of prod_ta)"
+    using trans_prod_finite by simp
+next
+  show "finite (range (inv_of prod_ta))"
+    using prod_inv_finite by simp
+next
+  from clk_set'_subs have "clk_set prod_ta \<subseteq> clk_set'" .
+  also have "\<dots> \<subseteq> {1..m}"
+    using clock_set unfolding clk_set'_def clkp_set'_def by force
+  finally show "clk_set prod_ta \<subseteq> {1..m}" .
+next
+  from clock_set have "\<forall>(_, d)\<in>clkp_set'. d \<in> \<nat>"
+    unfolding clkp_set'_def by force
+  then show "\<forall>(_, d)\<in>Timed_Automata.clkp_set prod_ta. d \<in> \<nat>"
+    by (auto dest!: subsetD[OF clkp_set'_subs])
+next
+  show "0 < m"
+    by (rule has_clock)
+qed
+
+end (* Simple Network Impl nat *)
+
+
+context Simple_Network_Impl
+begin
+
+definition "sem \<equiv> (set syncs, map (automaton_of o conv_automaton) automata, map_of bounds')"
+
+sublocale sem: Prod_TA_sem sem .
+
+lemma sem_N_eq:
+  "sem.N p = automaton_of (conv_automaton (automata ! p))" if \<open>p < n_ps\<close>
+  using that unfolding sem.N_def n_ps_def unfolding sem_def fst_conv snd_conv
+  by (subst nth_map) auto
+
+end (* Simple Network Impl *)
+
+inductive_cases step_u_elims:
+  "A \<turnstile> \<langle>L, s, u\<rangle> \<rightarrow>\<^bsub>Del\<^esub> \<langle>L', s', u'\<rangle>"
+  "A \<turnstile> \<langle>L, s, u\<rangle> \<rightarrow>\<^bsub>Internal a\<^esub> \<langle>L', s', u'\<rangle>"
+  "A \<turnstile> \<langle>L, s, u\<rangle> \<rightarrow>\<^bsub>Sync sync\<^esub> \<langle>L', s', u'\<rangle>"
+
+inductive_cases step_u_elims':
+  "(broadcast, N, B) \<turnstile> \<langle>L, s, u\<rangle> \<rightarrow>\<^bsub>Del\<^esub> \<langle>L', s', u'\<rangle>"
+  "(broadcast, N, B) \<turnstile> \<langle>L, s, u\<rangle> \<rightarrow>\<^bsub>Internal a\<^esub> \<langle>L', s', u'\<rangle>"
+  "(broadcast, N, B) \<turnstile> \<langle>L, s, u\<rangle> \<rightarrow>\<^bsub>Sync sync\<^esub> \<langle>L', s', u'\<rangle>"
+
+lemma (in Prod_TA_Defs) states_lengthD:
+  "length L = n_ps" if "L \<in> states"
+  using that unfolding states_def by simp
+
+end (* Theory *)
